\documentclass{ctexart}
\begin{document}



$$\Psi \left(\lambda \right) = \min_{p \in C}L \left(p, \lambda \right) = L \left(p_{\lambda}, \lambda \right) $$

$$ p_{\lambda} = \mathop{\arg\min}_{p \in C} L \left(p, \lambda \right)$$


$$\frac{\partial L \left(p,\lambda \right)}{\partial p \left(y|x\right)}  $$ 


$$ = \sum_{x, y \in \tau}\tilde{p} \left(x\right) \left(\log p \left(y|x\right) + 1 \right)  - \sum_{y}\lambda_{0}  -\sum_{i=1}^{n}\lambda_{i} \left( \sum_{x,y \in \tau} \tilde{p} \left(x\right) f_{i}(x,y) \right)    $$

$$ = \sum_{x, y \in \tau}\tilde{p} \left(x\right) \left(\log p \left(y|x\right) + 1 \right)  - \sum_{x} \tilde{p}(x)\sum_{y}\lambda_{0}  - \sum_{x,y \in \tau} \tilde{p}  \left(x\right) \left(  \sum_{i=1}^{n}\lambda_{i} f_{i}(x,y) \right)    $$

$$ = \sum_{x, y \in \tau}\tilde{p} (x) (\log p (y|x) + 1 ) - \sum_{x,y \in \tau} \tilde{p}(x)\lambda_{0} -  \sum_{x,y \in \tau} \tilde{p}  \left(x\right) \left(  \sum_{i=1}^{n}\lambda_{i} f_{i}(x,y) \right)$$

$$ = \sum_{x,y \in \tau} \tilde{p}(x) \left(   \log p \left(y|x\right) + 1 - \lambda_{0} - \sum_{i=1}^{n}\lambda_{i}f_{i}\left(x,y\right)           \right) = 0 $$

$$  p\left(y|x\right) = e^{\lambda_{0}-1}  e^{ \sum\limits_{i=1}^{n} \lambda_{i}  f_{i}\left(x,y\right)    }       $$
$$ \sum_y p \left(y|x\right) = e^{\lambda_{0}-1} \sum_y  e^{ \sum\limits_{i=1}^{n} \lambda_{i}  f_{i}\left(x,y\right)    }    = 1 $$

$$  e^{\lambda_{0}-1}  = \frac{1}{   \sum\limits_y  e^{ \sum\limits_{i=1}^{n} \lambda_{i}  f_{i}\left(x,y\right)    }    }  $$


$$   p\left(y|x\right) = \frac{1}{   \sum\limits_y  e^{ \sum\limits_{i=1}^{n} \lambda_{i}  f_{i}\left(x,y\right)    }    }  e^{ \sum\limits_{i=1}^{n} \lambda_{i}  f_{i}\left(x,y\right)    }     $$

$$ Z_{\lambda}\left(x\right) =       \sum_y  e^{ \sum\limits_{i=1}^{n} \lambda_{i}  f_{i}\left(x,y\right)    }    $$









\end{document}